[std/random/random_gen] -> [std/random/int]. [std/random/random_gen'] -> [std/random/random_int_in_range].

theories/std/random.v
@@ -11,7 +11,7 @@ From zoo Require Import
 Implicit Types t : val.
 
 Parameter random_create : val.
-Parameter random_gen : val.
+Parameter random_int : val.
 
 Parameter random_inv : ∀ `{zoo_G : !ZooG Σ}, val → iProp Σ.
 
@@ -29,46 +29,46 @@ Axiom random_create_spec : ∀ `{zoo_G : !ZooG Σ},
     random_inv t
   }}}.
 
-Axiom random_gen_spec : ∀ `{zoo_G : !ZooG Σ} t ub,
+Axiom random_int_spec : ∀ `{zoo_G : !ZooG Σ} t ub,
   (0 < ub)%Z →
   {{{
     random_inv t
   }}}
-    random_gen t #ub
+    random_int t #ub
   {{{ n,
     RET #n;
     ⌜0 ≤ n < ub⌝%Z
   }}}.
 
-Definition random_gen' : val :=
+Definition random_int_in_range : val :=
   fun: "t" "lb" "ub" =>
-    "lb" + random_gen "t" ("ub" - "lb").
+    "lb" + random_int "t" ("ub" - "lb").
 
 Section zoo_G.
   Context `{zoo_G : !ZooG Σ}.
 
-  Lemma random_gen_spec_nat t (ub : nat) :
+  Lemma random_int_spec_nat t (ub : nat) :
     0 < ub →
     {{{
       random_inv t
     }}}
-      random_gen t #ub
+      random_int t #ub
     {{{ n,
       RET #n;
       ⌜n < ub⌝
     }}}.
   Proof.
     iIntros "%Hub %Φ #Ht HΦ".
-    wp_apply (random_gen_spec with "Ht") as (n) "%Hn"; first lia.
+    wp_apply (random_int_spec with "Ht") as (n) "%Hn"; first lia.
     Z_to_nat n. iSteps.
   Qed.
 
-  Lemma random_gen'_spec t lb ub :
+  Lemma random_int_in_range_spec t lb ub :
     (lb < ub)%Z →
     {{{
       random_inv t
     }}}
-      random_gen' t #lb #ub
+      random_int_in_range t #lb #ub
     {{{ n,
       RET #n;
       ⌜lb ≤ n < ub⌝%Z
@@ -76,15 +76,15 @@ Section zoo_G.
   Proof.
     iIntros "%Hlt %Φ #Ht HΦ".
     wp_rec.
-    wp_smart_apply (random_gen_spec with "Ht") as "%n %Hn"; first lia.
+    wp_smart_apply (random_int_spec with "Ht") as "%n %Hn"; first lia.
     iSteps.
   Qed.
-  Lemma random_gen'_spec_nat t lb ub :
+  Lemma random_int_in_range_spec_nat t lb ub :
     lb < ub →
     {{{
       random_inv t
     }}}
-      random_gen' t #lb #ub
+      random_int_in_range t #lb #ub
     {{{ n,
       RET #n;
       ⌜lb ≤ n < ub⌝
@@ -92,10 +92,10 @@ Section zoo_G.
   Proof.
     iIntros "%Hlt %Φ Ht HΦ".
     wp_rec.
-    wp_smart_apply (random_gen_spec with "Ht") as "%n %Hn"; first lia.
+    wp_smart_apply (random_int_spec with "Ht") as "%n %Hn"; first lia.
     wp_pures.
     Z_to_nat n. rewrite -Nat2Z.inj_add. iSteps.
   Qed.
 End zoo_G.
 
-#[global] Opaque random_gen'.
+#[global] Opaque random_int_in_range.
